tests/lean/interactive/goal_info_rw.lean
@@ -1,0 +1,7 @@
+example (p q r : Prop) (h₁ : p = q) (h₂ : q = r) : p = r :=
+by rw [h₁,
+       --^ "command": "info"
+       -h₂,
+     --^ "command": "info"
+       -h₁]
+       --^ "command": "info"
